verified/sha/Seqs.s.dfy
@@ -1,0 +1,15 @@
+// REQUIRES-ANY: TEST, COLLECTIONS
+// RUN: %DAFNY /compile:0 %s %DARGS
+
+function last<T>(s:seq<T>):T
+    requires |s| > 0;
+{
+    s[|s|-1]
+}
+
+function all_but_last<T>(s:seq<T>):seq<T>
+    requires |s| > 0;
+    ensures  |all_but_last(s)| == |s| - 1;
+{
+    s[..|s|-1]
+}
