verified/sha/hmac_common.s.dfy
@@ -1,0 +1,28 @@
+// REQUIRES-ANY: TEST, SHA
+// RUN: %DAFNY /compile:0 %s %DARGS
+
+include "../words_and_bytes.s.dfy"
+include "../ARMdef.dfy"
+
+//-////////////////////////////////////////////////////////////////////////////
+//- HMAC specification based on:
+//- http://csrc.nist.gov/publications/fips/fips198-1/FIPS-198-1_final.pdf
+//-////////////////////////////////////////////////////////////////////////////
+
+function {:opaque} SeqXor(a:seq<word>, b:seq<word>) : seq<word>
+    requires |a|==|b|;
+    ensures  |SeqXor(a, b)| == |a|;
+    ensures  forall i :: 0 <= i < |a| ==> SeqXor(a, b)[i] == BitwiseXor(a[i], b[i]);
+{
+    if |a| == 0 then [] else [ BitwiseXor(a[0], b[0]) ] + SeqXor(a[1..], b[1..])
+}
+
+function {:autoReq} Opad(len:int) : seq<word>
+{
+    RepeatValue<word>(0x5c5c5c5c as word, len)
+}
+
+function {:autoReq} Ipad(len:int) : seq<word>
+{
+    RepeatValue<word>(0x36363636 as word, len)
+}
