verified/sha/sha256_context.i.dfy
@@ -1,0 +1,100 @@
+// REQUIRES-ANY: TEST, SHA
+// RUN: %DAFNY /compile:0 %s %DARGS
+
+include "sha256.i.dfy"
+include "../../Collections/Seqs.i.dfy"
+
+import opened Collections__Seqs_i_temp = Collections__Seqs_i
+
+///////////////////////////////////
+// FUNCTIONS
+///////////////////////////////////
+
+function ArrayToObject<T>(a:array<T>) : object
+{
+    a
+}
+
+function {:opaque} ToSeqUint8(s:seq<byte>) : seq<uint8>
+    ensures var s' := ToSeqUint8(s);
+            |s| == |s'|
+         && forall i :: 0 <= i < |s| ==> s[i] as uint8 == s'[i]
+{
+    if s == [] then []
+    else [s[0] as uint8] + ToSeqUint8(s[1..])
+}
+
+function {:opaque} ToSeqUint32(s:seq<uint>) : seq<uint32>
+    ensures var s' := ToSeqUint32(s);
+            |s| == |s'|
+         && forall i :: 0 <= i < |s| ==> s[i] as uint32 == s'[i]
+{
+    if s == [] then []
+    else [s[0] as uint32] + ToSeqUint32(s[1..])
+}
+
+///////////////////////////////////
+// TYPES
+///////////////////////////////////
+
+class SHA256Context
+{
+    ghost var z:SHA256Trace;
+    ghost var processed_bytes:seq<uint8>;
+    var H:array<uint>;
+    var unprocessed_bytes:array<byte>;
+    var num_unprocessed_bytes:uint;
+    var num_total_bytes:ulong;
+
+    ghost var Repr:set<object>;
+
+    function ToObject() : object
+    {
+        this
+    }
+
+    constructor()
+        modifies this;
+        ensures  fresh(this.H);
+        ensures  fresh(this.unprocessed_bytes);
+        ensures  Valid();
+    {
+        this.processed_bytes := [];
+        this.H := new uint[8];
+        this.unprocessed_bytes := new byte[64];
+        this.num_unprocessed_bytes := 0;
+        this.Repr := { ToObject(), ArrayToObject(this.H), ArrayToObject(this.unprocessed_bytes) };
+    }
+
+    predicate Valid()
+        reads this;
+    {
+           allocated(this.H)
+        && this.H.Length == 8
+        && allocated(this.unprocessed_bytes)
+        && this.unprocessed_bytes.Length == 64
+        && this.num_unprocessed_bytes as int <= 64
+        && this.Repr == { ToObject(), ArrayToObject(this.H), ArrayToObject(this.unprocessed_bytes) }
+    }
+
+    predicate ExportedInvariant()
+        reads this, Repr;
+    {
+           Valid()
+        && this.num_total_bytes as int == |this.processed_bytes| + (this.num_unprocessed_bytes as int)
+        && |this.processed_bytes| % 64 == 0
+        && this.num_unprocessed_bytes as int < 64
+        && this.num_total_bytes as int <= MaxBytesForSHA()
+        && IsCompleteSHA256Trace(this.z)
+        && SHA256TraceIsCorrect(this.z)
+        && WordSeqToBytes(ConcatenateSeqs(this.z.M)) == this.processed_bytes
+        && ToSeqUint32(this.H[..]) == last(this.z.H) 
+    }
+
+    function BytesIncluded() : seq<uint8>
+        requires Valid();
+        reads    this, Repr;
+    {
+        this.processed_bytes + ToSeqUint8(this.unprocessed_bytes[..this.num_unprocessed_bytes])
+    }
+}
