verified/sha/sha_common.s.dfy
@@ -1,0 +1,85 @@
+// REQUIRES-ANY: TEST, SHA
+// RUN: %DAFNY /compile:0 %s %DARGS
+
+//include "assembly.s.dfy"
+include "../words_and_bytes.s.dfy"
+include "../ARMdef.dfy"
+
+function method{:axiom} BitwiseAdd32(x:word, y:word):word
+    ensures BitwiseAdd32(x, y) == (((x as int) + (y as int)) % 0x100000000) as word;
+
+//-///////////////////////////////////////////////////
+//- Ch, Maj, BSIG0, BSIG1, SSIG0, SSIG1
+//-///////////////////////////////////////////////////
+
+function {:opaque} Ch(x:word, y:word, z:word) : word
+{
+    BitwiseXor(BitwiseAnd(x, y), BitwiseAnd(BitwiseNot(x), z))
+}
+
+function {:opaque} Maj(x:word, y:word, z:word) : word
+{
+    BitwiseXor(BitwiseXor(BitwiseAnd(x, y), BitwiseAnd(x, z)), BitwiseAnd(y, z))
+}
+
+function {:opaque} Parity(x:word, y:word, z:word) : word
+{
+    BitwiseXor(BitwiseXor(x, y), z)
+}
+
+function {:opaque} ft(t:word, x:word, y:word, z:word) : word
+    requires 0 <= t <= 79;
+{
+
+    if t >= 0 && t <= 19 then
+        Ch(x, y, z)
+
+    else if t >= 40 && t <= 59 then
+        Maj(x, y, z)
+    else
+        Parity(x, y, z)
+}
+
+function {:opaque} BSIG0(x:word) : word
+{
+    BitwiseXor(BitwiseXor(RotateRight(x, 2), RotateRight(x, 13)), RotateRight(x, 22))
+}
+
+function {:opaque} BSIG1(x:word) : word
+{
+    BitwiseXor(BitwiseXor(RotateRight(x, 6), RotateRight(x, 11)), RotateRight(x, 25))
+}
+
+function {:opaque} SSIG0(x:word) : word
+{
+    BitwiseXor(BitwiseXor(RotateRight(x, 7), RotateRight(x, 18)), RightShift(x, 3))
+}
+
+function {:opaque} SSIG1(x:word) : word
+{
+    BitwiseXor(BitwiseXor(RotateRight(x, 17), RotateRight(x, 19)), RightShift(x, 10))
+}
+
+function{:opaque} BreakIntoBlocks<T>(os:seq<T>, block_size:int) : seq<seq<T>>
+    requires 0 < block_size;
+    decreases |os|;
+{
+    if |os| == 0 then []
+    else if |os| < block_size then [os]
+    else [os[..block_size]] + BreakIntoBlocks(os[block_size..], block_size)
+}
+
+function MaxBytesForSHA() : int { 0x1FFF_FFFF_FFFF_FFFF }
+
+predicate WordSeqIsProperlySHAPaddedByteSeq(ws:seq<word>, bytes:seq<byte>)
+{
+       |bytes| <= MaxBytesForSHA()
+    && WordSeqToBytes(ws) == bytes + [0x80 as byte] + RepeatByte(0, (119 - (|bytes| % 64)) % 64) + Uint64ToBytes((|bytes| * 8) as uint64)
+}
+
+//- Used to avoid matching loops in some uses of forall
+//- (avoid formulas of the form "forall i :: ...a[i]...a[i+1]...", which can loop
+//- if the trigger is a[i] and the i+1 in the body is used to instantiate the i in the trigger)
+function TBlk(blk:int):bool { true }
+function TStep(t:word):bool { true }
+
